updated for new semantics

verif/Fib.v
@@ -14,18 +14,17 @@ Import ListNotations.
 
 (* Borrow from CompCert *)
 Require Import Coqlib.
-Require Import Integers.
+
+Require Import Bitvectors.
 
 Require Import AST.
 Require Import Semantics.
 Require Import Utils.
-Require Import Builtins.   
-        
-(* Grab some useful tactics : 
-  e: applies econstructor and some simplification whenever there is no choice to be made (not an If or Var) 
-  global: resolves the constructor for a var in the global env
-  localL resolves the constructor for a var in the local env  *)
-Require Import Tactics. 
+Require Import Builtins.
+Require Import BuiltinSem. 
+Require Import Values.    
+Require Import BuiltinSanity. 
+Require Import EvalTac. 
 
 (* right side of this generated from cryptol implementation *)
 
@@ -33,7 +32,71 @@ Import HaskellListNotations.
 
 
 
-(* 
+Definition fib_cry := [(NonRecursive (Decl (242,"demote") DPrim)),(NonRecursive (Decl (243,"+") DPrim)),(NonRecursive (Decl (244,"-") DPrim)),(NonRecursive (Decl (245,"*") DPrim)),(NonRecursive (Decl (246,"/") DPrim)),(NonRecursive (Decl (247,"%") DPrim)),(NonRecursive (Decl (248,"^^") DPrim)),(NonRecursive (Decl (249,"lg2") DPrim)),(NonRecursive (Decl (251,"True") DPrim)),(NonRecursive (Decl (252,"False") DPrim)),(NonRecursive (Decl (253,"negate") DPrim)),(NonRecursive (Decl (254,"complement") DPrim)),(NonRecursive (Decl (255,"<") DPrim)),(NonRecursive (Decl (256,">") DPrim)),(NonRecursive (Decl (257,"<=") DPrim)),(NonRecursive (Decl (258,">=") DPrim)),(NonRecursive (Decl (259,"==") DPrim)),(NonRecursive (Decl (260,"!=") DPrim)),(NonRecursive (Decl (261,"===") (DExpr (ETAbs (329,"a") (ETAbs (330,"b") (EAbs (331,"f") (EAbs (332,"g") (EAbs (333,"x") (EApp (EApp (ETApp (EVar (259,"==")) (TVar (TVBound 31 KType))) (EApp (EVar (331,"f")) (EVar (333,"x")))) (EApp (EVar (332,"g")) (EVar (333,"x")))))))))))),(NonRecursive (Decl (262,"!==") (DExpr (ETAbs (334,"a") (ETAbs (335,"b") (EAbs (336,"f") (EAbs (337,"g") (EAbs (338,"x") (EApp (EApp (ETApp (EVar (260,"!=")) (TVar (TVBound 41 KType))) (EApp (EVar (336,"f")) (EVar (338,"x")))) (EApp (EVar (337,"g")) (EVar (338,"x")))))))))))),(NonRecursive (Decl (263,"min") (DExpr (ETAbs (339,"a") (EAbs (340,"x") (EAbs (341,"y") (EIf (EApp (EApp (ETApp (EVar (255,"<")) (TVar (TVBound 50 KType))) (EVar (340,"x"))) (EVar (341,"y"))) (EVar (340,"x")) (EVar (341,"y"))))))))),(NonRecursive (Decl (264,"max") (DExpr (ETAbs (342,"a") (EAbs (343,"x") (EAbs (344,"y") (EIf (EApp (EApp (ETApp (EVar (256,">")) (TVar (TVBound 56 KType))) (EVar (343,"x"))) (EVar (344,"y"))) (EVar (343,"x")) (EVar (344,"y"))))))))),(NonRecursive (Decl (265,"/\\") (DExpr (EAbs (345,"x") (EAbs (346,"y") (EIf (EVar (345,"x")) (EVar (346,"y")) (EVar (252,"False")))))))),(NonRecursive (Decl (266,"\\/") (DExpr (EAbs (347,"x") (EAbs (348,"y") (EIf (EVar (347,"x")) (EVar (251,"True")) (EVar (348,"y")))))))),(NonRecursive (Decl (267,"==>") (DExpr (EAbs (349,"a") (EAbs (350,"b") (EIf (EVar (349,"a")) (EVar (350,"b")) (EVar (251,"True")))))))),(NonRecursive (Decl (268,"&&") DPrim)),(NonRecursive (Decl (269,"||") DPrim)),(NonRecursive (Decl (270,"^") DPrim)),(NonRecursive (Decl (271,"zero") DPrim)),(NonRecursive (Decl (272,"<<") DPrim)),(NonRecursive (Decl (273,">>") DPrim)),(NonRecursive (Decl (274,"<<<") DPrim)),(NonRecursive (Decl (275,">>>") DPrim)),(NonRecursive (Decl (276,"#") DPrim)),(NonRecursive (Decl (277,"splitAt") DPrim)),(NonRecursive (Decl (278,"join") DPrim)),(NonRecursive (Decl (279,"split") DPrim)),(NonRecursive (Decl (280,"reverse") DPrim)),(NonRecursive (Decl (281,"transpose") DPrim)),(NonRecursive (Decl (282,"@") DPrim)),(NonRecursive (Decl (283,"@@") DPrim)),(NonRecursive (Decl (284,"!") DPrim)),(NonRecursive (Decl (285,"!!") DPrim)),(NonRecursive (Decl (286,"update") DPrim)),(NonRecursive (Decl (287,"updateEnd") DPrim)),(NonRecursive (Decl (288,"updates") (DExpr (ETAbs (404,"a") (ETAbs (405,"b") (ETAbs (406,"c") (ETAbs (407,"d") (EAbs (408,"xs0") (EAbs (409,"idxs") (EAbs (410,"vals") (EWhere (EApp (EApp (ETApp (ETApp (ETApp (EVar (284,"!")) (TCon (TF TCAdd) [TCon (TC (TCNum 1)) [],TVar (TVBound 124 KNum)])) (TCon (TC TCSeq) [TVar (TVBound 121 KNum),TVar (TVBound 122 KType)])) (TCon (TC (TCNum 0)) [])) (EVar (411,"xss"))) (ETApp (ETApp (EVar (242,"demote")) (TCon (TC (TCNum 0)) [])) (TCon (TC (TCNum 0)) []))) [(Recursive [(Decl (411,"xss") (DExpr (EApp (EApp (ETApp (ETApp (ETApp (EVar (276,"#")) (TCon (TC (TCNum 1)) [])) (TVar (TVBound 124 KNum))) (TCon (TC TCSeq) [TVar (TVBound 121 KNum),TVar (TVBound 122 KType)])) (EList [(EVar (408,"xs0"))])) (EComp (EApp (EApp (EApp (ETApp (ETApp (ETApp (EVar (286,"update")) (TVar (TVBound 121 KNum))) (TVar (TVBound 122 KType))) (TVar (TVBound 123 KNum))) (EVar (412,"xs"))) (EVar (413,"i"))) (EVar (414,"b"))) [[(From (412,"xs") (EVar (411,"xss")))],[(From (413,"i") (EVar (409,"idxs")))],[(From (414,"b") (EVar (410,"vals")))]]))))])]))))))))))),(NonRecursive (Decl (289,"updatesEnd") (DExpr (ETAbs (415,"a") (ETAbs (416,"b") (ETAbs (417,"c") (ETAbs (418,"d") (EAbs (419,"xs0") (EAbs (420,"idxs") (EAbs (421,"vals") (EWhere (EApp (EApp (ETApp (ETApp (ETApp (EVar (284,"!")) (TCon (TF TCAdd) [TCon (TC (TCNum 1)) [],TVar (TVBound 159 KNum)])) (TCon (TC TCSeq) [TVar (TVBound 156 KNum),TVar (TVBound 157 KType)])) (TCon (TC (TCNum 0)) [])) (EVar (422,"xss"))) (ETApp (ETApp (EVar (242,"demote")) (TCon (TC (TCNum 0)) [])) (TCon (TC (TCNum 0)) []))) [(Recursive [(Decl (422,"xss") (DExpr (EApp (EApp (ETApp (ETApp (ETApp (EVar (276,"#")) (TCon (TC (TCNum 1)) [])) (TVar (TVBound 159 KNum))) (TCon (TC TCSeq) [TVar (TVBound 156 KNum),TVar (TVBound 157 KType)])) (EList [(EVar (419,"xs0"))])) (EComp (EApp (EApp (EApp (ETApp (ETApp (ETApp (EVar (287,"updateEnd")) (TVar (TVBound 156 KNum))) (TVar (TVBound 157 KType))) (TVar (TVBound 158 KNum))) (EVar (423,"xs"))) (EVar (424,"i"))) (EVar (425,"b"))) [[(From (423,"xs") (EVar (422,"xss")))],[(From (424,"i") (EVar (420,"idxs")))],[(From (425,"b") (EVar (421,"vals")))]]))))])]))))))))))),(NonRecursive (Decl (290,"fromThen") DPrim)),(NonRecursive (Decl (291,"fromTo") DPrim)),(NonRecursive (Decl (292,"fromThenTo") DPrim)),(NonRecursive (Decl (293,"infFrom") DPrim)),(NonRecursive (Decl (294,"infFromThen") DPrim)),(NonRecursive (Decl (295,"error") DPrim)),(NonRecursive (Decl (296,"pmult") DPrim)),(NonRecursive (Decl (297,"pdiv") DPrim)),(NonRecursive (Decl (298,"pmod") DPrim)),(NonRecursive (Decl (299,"random") DPrim)),(NonRecursive (Decl (303,"take") (DExpr (ETAbs (451,"front") (ETAbs (452,"back") (ETAbs (453,"elem") (EAbs (454,"__p1") (EWhere (EVar (456,"x")) [(NonRecursive (Decl (455,"__p2") (DExpr (EApp (ETApp (ETApp (ETApp (EVar (277,"splitAt")) (TVar (TVBound 214 KNum))) (TVar (TVBound 215 KNum))) (TVar (TVBound 216 KType))) (EVar (454,"__p1")))))),(NonRecursive (Decl (456,"x") (DExpr (ESel (EVar (455,"__p2")) (TupleSel 0))))),(NonRecursive (Decl (457,"__p0") (DExpr (ESel (EVar (455,"__p2")) (TupleSel 1)))))])))))))),(NonRecursive (Decl (304,"drop") (DExpr (ETAbs (458,"front") (ETAbs (459,"back") (ETAbs (460,"elem") (EAbs (461,"__p4") (EWhere (EVar (464,"y")) [(NonRecursive (Decl (462,"__p5") (DExpr (EApp (ETApp (ETApp (ETApp (EVar (277,"splitAt")) (TVar (TVBound 231 KNum))) (TVar (TVBound 232 KNum))) (TVar (TVBound 233 KType))) (EVar (461,"__p4")))))),(NonRecursive (Decl (463,"__p3") (DExpr (ESel (EVar (462,"__p5")) (TupleSel 0))))),(NonRecursive (Decl (464,"y") (DExpr (ESel (EVar (462,"__p5")) (TupleSel 1)))))])))))))),(NonRecursive (Decl (305,"tail") (DExpr (ETAbs (465,"a") (ETAbs (466,"b") (EAbs (467,"xs") (EApp (ETApp (ETApp (ETApp (EVar (304,"drop")) (TCon (TC (TCNum 1)) [])) (TVar (TVBound 249 KNum))) (TVar (TVBound 250 KType))) (EVar (467,"xs"))))))))),(NonRecursive (Decl (306,"width") (DExpr (ETAbs (468,"bits") (ETAbs (469,"len") (ETAbs (470,"elem") (EAbs (471,"__p6") (ETApp (ETApp (EVar (242,"demote")) (TVar (TVBound 256 KNum))) (TVar (TVBound 255 KNum)))))))))),(NonRecursive (Decl (307,"undefined") (DExpr (ETAbs (472,"a") (EApp (ETApp (ETApp (EVar (295,"error")) (TVar (TVBound 260 KType))) (TCon (TC (TCNum 9)) [])) (EList [(ETApp (ETApp (EVar (242,"demote")) (TCon (TC (TCNum 117)) [])) (TCon (TC (TCNum 8)) [])),(ETApp (ETApp (EVar (242,"demote")) (TCon (TC (TCNum 110)) [])) (TCon (TC (TCNum 8)) [])),(ETApp (ETApp (EVar (242,"demote")) (TCon (TC (TCNum 100)) [])) (TCon (TC (TCNum 8)) [])),(ETApp (ETApp (EVar (242,"demote")) (TCon (TC (TCNum 101)) [])) (TCon (TC (TCNum 8)) [])),(ETApp (ETApp (EVar (242,"demote")) (TCon (TC (TCNum 102)) [])) (TCon (TC (TCNum 8)) [])),(ETApp (ETApp (EVar (242,"demote")) (TCon (TC (TCNum 105)) [])) (TCon (TC (TCNum 8)) [])),(ETApp (ETApp (EVar (242,"demote")) (TCon (TC (TCNum 110)) [])) (TCon (TC (TCNum 8)) [])),(ETApp (ETApp (EVar (242,"demote")) (TCon (TC (TCNum 101)) [])) (TCon (TC (TCNum 8)) [])),(ETApp (ETApp (EVar (242,"demote")) (TCon (TC (TCNum 100)) [])) (TCon (TC (TCNum 8)) []))])))))),(NonRecursive (Decl (308,"groupBy") (DExpr (ETAbs (473,"each") (ETAbs (474,"parts") (ETAbs (475,"elem") (ETApp (ETApp (ETApp (EVar (279,"split")) (TVar (TVBound 266 KNum))) (TVar (TVBound 265 KNum))) (TVar (TVBound 267 KType))))))))),(NonRecursive (Decl (310,"trace") DPrim)),(NonRecursive (Decl (311,"traceVal") (DExpr (ETAbs (480,"n") (ETAbs (481,"a") (EAbs (482,"msg") (EAbs (483,"x") (EApp (EApp (EApp (ETApp (ETApp (ETApp (EVar (310,"trace")) (TVar (TVBound 273 KNum))) (TVar (TVBound 274 KType))) (TVar (TVBound 274 KType))) (EVar (482,"msg"))) (EVar (483,"x"))) (EVar (483,"x")))))))))),(Recursive [(Decl (484,"fib") (DExpr (EAbs (485,"n") (EIf (EApp (EApp (ETApp (EVar (259,"==")) (TCon (TC TCSeq) [TCon (TC (TCNum 32)) [],TCon (TC TCBit) []])) (EVar (485,"n"))) (ETApp (ETApp (EVar (242,"demote")) (TCon (TC (TCNum 0)) [])) (TCon (TC (TCNum 32)) []))) (ETApp (ETApp (EVar (242,"demote")) (TCon (TC (TCNum 1)) [])) (TCon (TC (TCNum 32)) [])) (EIf (EApp (EApp (ETApp (EVar (259,"==")) (TCon (TC TCSeq) [TCon (TC (TCNum 32)) [],TCon (TC TCBit) []])) (EVar (485,"n"))) (ETApp (ETApp (EVar (242,"demote")) (TCon (TC (TCNum 1)) [])) (TCon (TC (TCNum 32)) []))) (ETApp (ETApp (EVar (242,"demote")) (TCon (TC (TCNum 1)) [])) (TCon (TC (TCNum 32)) [])) (EApp (EApp (ETApp (EVar (243,"+")) (TCon (TC TCSeq) [TCon (TC (TCNum 32)) [],TCon (TC TCBit) []])) (EApp (EVar (484,"fib")) (EApp (EApp (ETApp (EVar (243,"+")) (TCon (TC TCSeq) [TCon (TC (TCNum 32)) [],TCon (TC TCBit) []])) (EVar (485,"n"))) (EApp (ETApp (EVar (253,"negate")) (TCon (TC TCSeq) [TCon (TC (TCNum 32)) [],TCon (TC TCBit) []])) (ETApp (ETApp (EVar (242,"demote")) (TCon (TC (TCNum 1)) [])) (TCon (TC (TCNum 32)) [])))))) (EApp (EVar (484,"fib")) (EApp (EApp (ETApp (EVar (243,"+")) (TCon (TC TCSeq) [TCon (TC (TCNum 32)) [],TCon (TC TCBit) []])) (EVar (485,"n"))) (EApp (ETApp (EVar (253,"negate")) (TCon (TC TCSeq) [TCon (TC (TCNum 32)) [],TCon (TC TCBit) []])) (ETApp (ETApp (EVar (242,"demote")) (TCon (TC (TCNum 2)) [])) (TCon (TC (TCNum 32)) [])))))))))))])].
+
+Definition width : nat := 32. 
+Definition fibident : ident := (484, "fib"). 
+Definition fibvar : ident := (12, "var"). 
+
+Lemma nz : width <> O.
+Proof. 
+  unfold width. congruence. 
+Qed.
+
+
+(* Global environment *)
+Definition fib_ge := bind_decl_groups fib_cry gempty. 
+
+
+Definition nz32 (n:Z) := bits (@repr width nz n). 
+Definition Env (n:Z) := extend empty fibvar (nz32 n). 
+
+Definition E := Env 0. 
+
+(* Fib 0 = 1 *)
+Lemma eval_fib0 : eval_expr fib_ge E (EApp (EVar fibident) (EVar fibvar)) (nz32 1).
+Proof. 
+  e. e. e. e. e. e. e. e. e. e. e. e. e. e. e. e. e. e. e. e. e. e. e. e. e. e. 
+  e. e. e. e. e. e. e. e. e. e. e. e. e. e. e. e. e. e. e. e. 
+  (* lol *)
+  Unshelve. exact nz. 
+Qed. 
+
+Definition E1 := Env 1.
+ 
+(* Fib 1 = 1 *) 
+Lemma eval_fib1 : eval_expr fib_ge E1 (EApp (EVar fibident) (EVar fibvar)) (nz32 1). 
+Proof. 
+  repeat e.
+
+  Unshelve. all: exact nz.
+Qed. 
+
+Definition E3 := Env 3.
+
+(* Fib 3 = 3 *) 
+Lemma eval_fib3 : eval_expr fib_ge E3 (EApp (EVar fibident) (EVar fibvar)) (nz32 3).
+Proof. 
+  repeat e. (* Takes like 10 min *)
+
+  Unshelve. all: exact nz. 
+Qed.  
+  
+
+
+
+
+
+
+
+
+(*  Old version before Semantics.v changes
+
+
+(* Grab some useful tactics : 
+  e: applies econstructor and some simplification whenever there is no choice to be made (not an If or Var) 
+  global: resolves the constructor for a var in the global env
+  local: resolves the constructor for a var in the local env  *)
 
 (* right side of this generated from cryptol implementation Fib.cry *)
 
